refacot(Modal): Refactor Logics (#365)

Foundation/Modal/Hilbert/S5Grz.lean
@@ -49,11 +49,13 @@ end S5Grz
 end LO.Entailment
 
 
-namespace LO.Modal.Hilbert
+namespace LO.Modal
 
 open Entailment
 
-protected abbrev S5Grz : Hilbert ℕ := ⟨{Axioms.K (.atom 0) (.atom 1), Axioms.T (.atom 0), Axioms.Five (.atom 0), Axioms.Grz (.atom 0)}⟩
+protected abbrev Hilbert.S5Grz : Hilbert ℕ := ⟨{Axioms.K (.atom 0) (.atom 1), Axioms.T (.atom 0), Axioms.Five (.atom 0), Axioms.Grz (.atom 0)}⟩
+
+namespace Hilbert.S5Grz
 instance : (Hilbert.S5Grz).HasK where p := 0; q := 1;
 instance : (Hilbert.S5Grz).HasT where p := 0
 instance : (Hilbert.S5Grz).HasFive where p := 0
@@ -61,11 +63,19 @@ instance : (Hilbert.S5Grz).HasGrz where p := 0
 instance : Entailment.Modal.S5Grz (Hilbert.S5Grz) where
 instance : Entailment.Modal.KTc' (Hilbert.S5Grz) where
 
-theorem iff_provable_S5Grz_provable_Triv : (Hilbert.S5Grz ⊢! φ) ↔ (Hilbert.Triv ⊢! φ) := by
+end Hilbert.S5Grz
+
+protected abbrev Logic.S5Grz := Hilbert.S5Grz.logic
+
+theorem Hilbert.iff_provable_S5Grz_provable_Triv : (Hilbert.S5Grz ⊢! φ) ↔ (Hilbert.Triv ⊢! φ) := by
   constructor;
   . apply fun h ↦ (weakerThan_of_dominate_axioms @h).subset;
     simp;
   . apply fun h ↦ (weakerThan_of_dominate_axioms @h).subset;
     rintro φ (⟨_, _, rfl⟩ | (⟨_, rfl⟩ | ⟨_, rfl⟩)) <;> simp;
 
-end LO.Modal.Hilbert
+lemma Logic.eq_S5Grz_Triv : Logic.S5Grz = Logic.Triv := by
+  ext φ;
+  exact Hilbert.iff_provable_S5Grz_provable_Triv;
+
+end LO.Modal
