Foundation.lean
@@ -60,10 +60,10 @@ import Foundation.Modal.Hilbert.KP
 import Foundation.Modal.Hilbert.S5Grz
 import Foundation.Modal.Hilbert.GL.Alternatives
 
-import Foundation.Modal.Kripke.Hilbert.GL.Unnecessitation
-import Foundation.Modal.Kripke.Hilbert.GL.MDP
+import Foundation.Modal.Kripke.Logic.GL.Unnecessitation
+import Foundation.Modal.Kripke.Logic.GL.MDP
 
-import Foundation.Modal.Kripke.Hilbert.Grz.Completeness
+import Foundation.Modal.Kripke.Logic.Grz.Completeness
 
 import Foundation.Modal.Kripke.NNFormula
 import Foundation.Modal.Kripke.ComplexityLimited
@@ -81,18 +81,8 @@ import Foundation.Modal.ModalCompanion.Cl
 import Foundation.Modal.Boxdot.K4_S4
 import Foundation.Modal.Boxdot.GL_Grz
 
-import Foundation.Modal.Logic.WellKnown
-import Foundation.Modal.Logic.Extension
 
-import Foundation.Modal.Logic.Sublogic.ModalCube
-import Foundation.Modal.Logic.Sublogic.GL
-import Foundation.Modal.Logic.Sublogic.Grz
-import Foundation.Modal.Logic.Sublogic.K4
-import Foundation.Modal.Logic.Sublogic.KH
-import Foundation.Modal.Logic.Sublogic.KTc
-import Foundation.Modal.Logic.Sublogic.S4
-import Foundation.Modal.Logic.Sublogic.S5Grz
-import Foundation.Modal.Logic.Sublogic.Trivials
+import Foundation.Modal.Logic.Extension
 
 import Foundation.Modal.Logic.S.Consistent
 
