Foundation/Modal/Boxdot/GL_Grz.lean
@@ -1,14 +1,11 @@
 import Foundation.Modal.Boxdot.Basic
-import Foundation.Modal.Logic.WellKnown
+import Foundation.Modal.Kripke.Logic.GL.Completeness
+import Foundation.Modal.Kripke.Logic.Grz.Completeness
 
 namespace LO.Modal
 
+
 namespace Kripke
-
-open Relation (ReflGen)
-open Formula.Kripke
-
-variable {F : Frame} {φ : Formula _}
 
 lemma mem_reflClosure_GrzFiniteFrameClass_of_mem_GLFiniteFrameClass (hF : F ∈ FrameClass.finite_trans_irrefl) : F^= ∈ FrameClass.finite_partial_order := by
   obtain ⟨_, _, _⟩ := hF;
@@ -17,71 +14,6 @@ lemma mem_reflClosure_GrzFiniteFrameClass_of_mem_GLFiniteFrameClass (hF : F ∈ 
 lemma mem_irreflClosure_GLFiniteFrameClass_of_mem_GrzFiniteFrameClass (hF : F ∈ FrameClass.finite_partial_order) : F^≠ ∈ FrameClass.finite_trans_irrefl := by
   obtain ⟨_, _, F_trans, F_antisymm⟩ := hF;
   refine ⟨inferInstance, inferInstance, inferInstance⟩;
-
-lemma iff_boxdot_reflexive_closure : (Satisfies ⟨F, V⟩ x (φᵇ)) ↔ (Satisfies ⟨F^=, V⟩ x φ) := by
-  induction φ generalizing x with
-  | himp φ ψ ihp ihq =>
-    constructor;
-    . intro h hp;
-      apply ihq.mp;
-      exact h $ ihp.mpr hp;
-    . intro h hp;
-      apply ihq.mpr;
-      exact h $ ihp.mp hp;
-  | hbox φ ih =>
-    simp [Formula.BoxdotTranslation, Box.boxdot, Satisfies];
-    constructor;
-    . rintro ⟨h₁, h₂⟩;
-      intro y Rxy;
-      rcases (Relation.reflGen_iff _ _ _ |>.mp Rxy) with (rfl | Rxy);
-      . apply ih.mp h₁;
-      . exact ih.mp $ h₂ y Rxy;
-    . rintro h;
-      constructor;
-      . exact ih.mpr $ @h x ReflGen.refl;
-      . intro y Rxy;
-        apply ih.mpr;
-        exact @h y (ReflGen.single Rxy);
-  | _ => rfl;
-
-lemma iff_frame_boxdot_reflexive_closure : (F ⊧ (φᵇ)) ↔ ((F^=) ⊧ φ) := by
-  constructor;
-  . intro h V x; apply iff_boxdot_reflexive_closure.mp; exact h V x;
-  . intro h V x; apply iff_boxdot_reflexive_closure.mpr; exact h V x;
-
-lemma iff_reflexivize_irreflexivize [IsRefl _ F] {x : F.World} {V} : (Satisfies ⟨F, V⟩ x φ) ↔ (Satisfies ⟨F^≠^=, V⟩ x φ) := by
-  induction φ generalizing x with
-  | hatom φ => rfl;
-  | hfalsum => rfl;
-  | himp φ ψ ihp ihq =>
-    constructor;
-    . intro h hp;
-      apply ihq.mp;
-      exact h $ ihp.mpr hp;
-    . intro h hp;
-      apply ihq.mpr;
-      exact h $ ihp.mp hp;
-  | hbox φ ihp =>
-    constructor;
-    . intro h y Rxy;
-      apply ihp (x := y) |>.mp;
-      exact h y $ by
-        induction Rxy with
-        | refl => apply IsRefl.refl;
-        | single h => exact h.2;
-    . intro h y Rxy;
-      by_cases e : x = y;
-      . subst e;
-        apply ihp.mpr;
-        exact h x ReflGen.refl;
-      . apply ihp (x := y) |>.mpr;
-        exact h y $ by
-          exact ReflGen.single ⟨(by simpa), Rxy⟩;
-
-lemma iff_reflexivize_irreflexivize' [IsRefl _ F] : (F ⊧ φ) ↔ ((F^≠^=) ⊧ φ) := by
-  constructor;
-  . intro h V x; apply iff_reflexivize_irreflexivize.mp; exact h V x;
-  . intro h V x; apply iff_reflexivize_irreflexivize.mpr; exact h V x;
 
 end Kripke
 
