Foundation/Modal/Kripke/Logic/GrzPoint3.lean
@@ -1,0 +1,154 @@
+import Foundation.Modal.Kripke.Logic.GrzPoint2
+import Foundation.Modal.Kripke.Logic.S4Point3
+
+namespace LO.Modal
+
+open Formula
+open Formula.Kripke
+open Entailment
+open Entailment.Context
+open Kripke
+
+
+open Entailment
+open Entailment.Context
+open Formula
+open Formula.Kripke
+open Hilbert.Kripke
+open Kripke
+
+namespace Kripke
+
+abbrev FrameClass.finite_connected_partial_order : FrameClass := { F | F.IsFinite ∧ IsPartialOrder _ F.Rel ∧ IsConnected _ F.Rel  }
+
+end Kripke
+
+
+namespace Hilbert.GrzPoint3.Kripke
+
+instance finite_sound : Sound (Hilbert.GrzPoint3) FrameClass.finite_connected_partial_order := instSound_of_validates_axioms $ by
+  apply FrameClass.Validates.withAxiomK;
+  rintro F ⟨_, _, _⟩ _ (rfl | rfl);
+  . exact validate_AxiomGrz_of_finite_strict_preorder;
+  . exact validate_AxiomPoint3_of_connected;
+
+instance consistent : Entailment.Consistent (Hilbert.GrzPoint3) :=
+  consistent_of_sound_frameclass FrameClass.finite_connected_partial_order $ by
+    use whitepoint;
+    refine ⟨inferInstance, inferInstance, inferInstance⟩;
+
+instance finite_complete : Complete (Hilbert.GrzPoint3) (FrameClass.finite_connected_partial_order) :=
+  Kripke.Grz.complete_of_mem_miniCanonicalFrame FrameClass.finite_connected_partial_order $ by
+    sorry;
+    /-
+    intro φ;
+    refine ⟨miniCanonicalFrame.reflexive, miniCanonicalFrame.transitive, miniCanonicalFrame.antisymm, ?_⟩;
+    intro x y z ⟨⟨Rxy₁, Rxy₂⟩, ⟨Rxz₁, Rxz₂⟩⟩;
+    apply or_iff_not_imp_left.mpr;
+    intro nRyz;
+    rcases (not_and_or.mp nRyz) with (nRyz | nRyz);
+    . push_neg at nRyz;
+      obtain ⟨ψ, hψ, ⟨hψy, hψz⟩⟩ := nRyz;
+      constructor;
+      . intro ξ hξ₁ hξ₂;
+        apply Rxy₁;
+        . exact hξ₁;
+        . sorry;
+      . intro hyz;
+        have exy := Rxy₂ ?_;
+        have exz := Rxz₂ ?_;
+        tauto;
+        . subst exy;
+          intro ξ hξ hξz;
+          sorry;
+        . intro ξ hξ hξy;
+          sorry;
+    . push_neg at nRyz;
+      replace ⟨nRyz₁, nRyz₂⟩ := nRyz;
+      constructor;
+      . sorry;
+      . sorry;
+    -/
+
+end Hilbert.GrzPoint3.Kripke
+
+namespace Logic
+
+open Formula
+open Entailment
+open Kripke
+
+lemma GrzPoint3.Kripke.finite_connected_partial_order : Logic.GrzPoint3 = FrameClass.finite_connected_partial_order.logic := eq_hilbert_logic_frameClass_logic
+
+instance : ProperSublogic Logic.GrzPoint2 Logic.GrzPoint3 := ⟨by
+  constructor;
+  . rw [GrzPoint2.Kripke.finite_confluent_partial_order, GrzPoint3.Kripke.finite_connected_partial_order];
+    rintro φ hφ F ⟨_, _, _⟩;
+    apply hφ;
+    refine ⟨by tauto, inferInstance, inferInstance⟩;
+  . suffices ∃ φ, Hilbert.GrzPoint3 ⊢! φ ∧ ¬FrameClass.finite_confluent_partial_order ⊧ φ by
+      rw [GrzPoint2.Kripke.finite_confluent_partial_order];
+      tauto;
+    use Axioms.Point3 (.atom 0) (.atom 1);
+    constructor;
+    . simp;
+    . apply Kripke.not_validOnFrameClass_of_exists_model_world;
+      let F : Frame := ⟨Fin 4, λ x y => x = 0 ∨ x = y ∨ y = 3⟩;
+      let M : Model := ⟨
+        F,
+        λ x a => match a with | 0 => (1 : F.World) ≺ x | 1 => (2 : F.World) ≺ x | _ => False
+      ⟩;
+      use M, 0;
+      constructor;
+      . refine ⟨by tauto, {
+          refl := by omega,
+          trans := by omega,
+          antisymm := by simp [M, F]; omega,
+        }, ⟨?_⟩⟩;
+        . rintro x y z ⟨(_ | _ | Rxy), (_ | _ | Rxy)⟩;
+          repeat { use 3; tauto; }
+      . apply Satisfies.or_def.not.mpr
+        push_neg;
+        constructor;
+        . apply Satisfies.box_def.not.mpr;
+          push_neg;
+          use 1;
+          constructor;
+          . tauto;
+          . apply Satisfies.imp_def₂.not.mpr;
+            push_neg;
+            constructor;
+            . tauto;
+            . simp [M, Semantics.Realize, Satisfies, Frame.Rel', F];
+        . apply Satisfies.box_def.not.mpr;
+          push_neg;
+          use 2;
+          constructor;
+          . tauto;
+          . apply Satisfies.imp_def₂.not.mpr;
+            push_neg;
+            constructor;
+            . tauto;
+            . simp [M, Semantics.Realize, Satisfies, Frame.Rel', F];
+⟩
+
+instance : ProperSublogic Logic.S4Point3 Logic.GrzPoint3 := ⟨by
+  constructor;
+  . exact Hilbert.weakerThan_of_dominate_axioms (by simp) |>.subset;
+  . suffices ∃ φ, Hilbert.GrzPoint3 ⊢! φ ∧ ¬FrameClass.finite_connected_preorder ⊧ φ by
+      rw [S4Point3.Kripke.finite_connected_preorder];
+      tauto;
+    use Axioms.Grz (.atom 0);
+    constructor;
+    . simp;
+    . apply Kripke.not_validOnFrameClass_of_exists_model_world;
+      use ⟨⟨Fin 2, λ x y => True⟩, λ w _ => w = 1⟩, 0;
+      constructor;
+      . refine ⟨inferInstance, {refl := by simp, trans := by simp}, ⟨by simp [Connected]⟩⟩;
+      . simp [Reflexive, Transitive, Semantics.Realize, Satisfies];
+⟩
+
+end Logic
+
+
+end LO.Modal
