Foundation/Modal/Kripke/Logic/K4.lean
@@ -1,0 +1,87 @@
+import Foundation.Modal.Hilbert.WellKnown
+import Foundation.Modal.Kripke.AxiomGeach
+import Foundation.Modal.Kripke.Hilbert
+import Foundation.Modal.Kripke.Filtration
+import Foundation.Modal.Kripke.Logic.K
+
+namespace LO.Modal
+
+open Kripke
+open Hilbert.Kripke
+open Geachean
+
+protected abbrev Kripke.FrameClass.trans : FrameClass := { F | IsTrans _ F }
+protected abbrev Kripke.FrameClass.finite_trans : FrameClass := { F | Finite F ∧ IsTrans _ F }
+
+namespace Hilbert.K4.Kripke
+
+instance sound : Sound (Hilbert.K4) Kripke.FrameClass.trans := instSound_of_validates_axioms $ by
+  apply FrameClass.Validates.withAxiomK;
+  rintro F F_trans φ rfl;
+  apply validate_AxiomFour_of_transitive (trans := F_trans);
+
+instance consistent : Entailment.Consistent (Hilbert.K4) :=
+  consistent_of_sound_frameclass FrameClass.trans $ by
+    use whitepoint;
+    apply Set.mem_setOf_eq.mpr;
+    infer_instance;
+
+instance canonical : Canonical (Hilbert.K4) Kripke.FrameClass.trans := ⟨by
+  apply Set.mem_setOf_eq.mpr;
+  infer_instance;
+⟩
+
+instance complete : Complete (Hilbert.K4) Kripke.FrameClass.trans := inferInstance
+
+open finestFiltrationTransitiveClosureModel in
+instance finite_complete : Complete (Hilbert.K4) Kripke.FrameClass.finite_trans := ⟨by
+  intro φ hp;
+  apply Kripke.complete.complete;
+  intro F F_trans V x;
+  replace F_trans := Set.mem_setOf_eq.mp F_trans;
+  let M : Kripke.Model := ⟨F, V⟩;
+  let FM := finestFiltrationTransitiveClosureModel M φ.subformulas;
+  apply filtration FM (finestFiltrationTransitiveClosureModel.filterOf) (by subformula) |>.mpr;
+  apply hp;
+  refine ⟨?_, inferInstance⟩;
+  . apply FilterEqvQuotient.finite;
+    simp;
+⟩
+
+end Hilbert.K4.Kripke
+
+namespace Logic
+
+open Formula
+open Entailment
+open Kripke
+
+lemma K4.Kripke.trans : Logic.K4 = FrameClass.trans.logic := eq_hilbert_logic_frameClass_logic
+
+instance : ProperSublogic Logic.K Logic.K4 := ⟨by
+  constructor;
+  . exact Hilbert.weakerThan_of_dominate_axioms (by simp) |>.subset;
+  . suffices ∃ φ, Hilbert.K4 ⊢! φ ∧ ¬FrameClass.all ⊧ φ by
+      rw [K.Kripke.all];
+      tauto;
+    use (Axioms.Four (.atom 0));
+    constructor;
+    . exact axiomFour!;
+    . apply Kripke.not_validOnFrameClass_of_exists_model_world;
+      let M : Model := ⟨⟨Fin 2, λ x y => x ≠ y⟩, λ w _ => w = 1⟩;
+      use M, 0;
+      constructor
+      . trivial;
+      . suffices (∀ (y : M.World), (0 : M.World) ≺ y → y = 1) ∧ ∃ x, (0 : M.World) ≺ x ∧ ∃ y, x ≺ y ∧ y ≠ 1 by
+          simpa [Semantics.Realize, Satisfies];
+        constructor;
+        . intro x;
+          match x with
+          | 0 => tauto;
+          | 1 => tauto;
+        . exact ⟨1, by omega, 0, by omega, by trivial⟩;
+⟩
+
+end Logic
+
+end LO.Modal
