Foundation/Modal/Kripke/Logic/K45.lean
@@ -1,0 +1,97 @@
+import Foundation.Modal.Kripke.AxiomGeach
+import Foundation.Modal.Kripke.Hilbert
+import Foundation.Modal.Hilbert.WellKnown
+import Foundation.Modal.Kripke.Logic.K4
+import Foundation.Modal.Kripke.Logic.K4Point3
+import Foundation.Modal.Kripke.Logic.K5
+
+namespace LO.Modal
+
+open Kripke
+open Hilbert.Kripke
+open Geachean
+
+protected abbrev Kripke.FrameClass.trans_eucl : FrameClass := { F | IsTrans _ F ∧ IsEuclidean _ F }
+
+namespace Hilbert.K45.Kripke
+
+instance sound : Sound (Hilbert.K45) FrameClass.trans_eucl := instSound_of_validates_axioms $ by
+  apply FrameClass.Validates.withAxiomK;
+  rintro F ⟨_, _⟩ _ (rfl | rfl);
+  . exact validate_AxiomFour_of_transitive;
+  . exact validate_AxiomFive_of_euclidean;
+
+instance consistent : Entailment.Consistent (Hilbert.K45) := consistent_of_sound_frameclass Kripke.FrameClass.trans_eucl $ by
+  use whitepoint;
+  constructor <;> infer_instance;
+
+instance canonical : Canonical (Hilbert.K45) FrameClass.trans_eucl := ⟨by
+  apply Set.mem_setOf_eq.mpr;
+  constructor <;> infer_instance;
+⟩
+
+instance complete : Complete (Hilbert.K45) FrameClass.trans_eucl := inferInstance
+
+end Hilbert.K45.Kripke
+
+
+namespace Logic
+
+open Formula
+open Entailment
+open Kripke
+
+lemma K45.Kripke.trans_eucl : Logic.K45 = FrameClass.trans_eucl.logic := eq_hilbert_logic_frameClass_logic
+
+instance : ProperSublogic Logic.K5 Logic.K45 := ⟨by
+  constructor;
+  . exact Hilbert.weakerThan_of_dominate_axioms (by simp) |>.subset;
+  . suffices ∃ φ, Hilbert.K45 ⊢! φ ∧ ¬Kripke.FrameClass.eucl ⊧ φ by
+      rw [K5.Kripke.eucl];
+      tauto;
+    use (Axioms.Four (.atom 0));
+    constructor;
+    . exact axiomFour!;
+    . apply Kripke.not_validOnFrameClass_of_exists_model_world;
+      let M : Model := ⟨⟨Fin 3, λ x y => (x = 0 ∧ y = 1) ∨ (x ≠ 0 ∧ y ≠ 0)⟩, λ w _ => w = 1⟩;
+      use M, 0;
+      constructor;
+      . refine ⟨by unfold Euclidean; omega⟩;
+      . suffices (∀ (y : M.World), (0 : M.World) ≺ y → y = 1) ∧ ∃ x, (0 : M.World) ≺ x ∧ ∃ z, x ≺ z ∧ ¬z = 1 by
+          simpa [M, Semantics.Realize, Satisfies];
+        constructor;
+        . intro y; tauto;
+        . exact ⟨1, by omega, 2, by omega, by trivial⟩;
+⟩
+
+instance : ProperSublogic Logic.K4Point3 Logic.K45 := ⟨by
+  constructor;
+  . rw [K4Point3.Kripke.trans_weakConnected, K45.Kripke.trans_eucl];
+    rintro φ hφ F ⟨_, _⟩;
+    apply hφ;
+    refine ⟨inferInstance, inferInstance⟩;
+  . suffices ∃ φ, Hilbert.K45 ⊢! φ ∧ ¬Kripke.FrameClass.trans_weakConnected ⊧ φ by
+      rw [K4Point3.Kripke.trans_weakConnected];
+      tauto;
+    use (Axioms.Five (.atom 0));
+    constructor;
+    . simp;
+    . apply Kripke.not_validOnFrameClass_of_exists_model_world;
+      let M : Model := ⟨
+        ⟨Fin 3, λ x y => x < y⟩,
+        λ w a => w = 2
+      ⟩;
+      use M, 0;
+      constructor;
+      . refine ⟨⟨by omega⟩, ⟨by simp [M, WeakConnected]⟩⟩
+      . suffices (0 : M.World) ≺ 2 ∧ ∃ x, (0 : M.World) ≺ x ∧ ¬x ≺ 2 by
+          simpa [M, Semantics.Realize, Satisfies];
+        constructor;
+        . omega;
+        . use 2;
+          omega;
+⟩
+
+end Logic
+
+end LO.Modal
