Foundation/Modal/Kripke/Logic/K4Point1.lean
@@ -1,0 +1,63 @@
+import Foundation.Modal.Kripke.Logic.K4
+import Foundation.Modal.Kripke.AxiomM
+
+namespace LO.Modal
+
+open Kripke
+open Hilbert.Kripke
+open Geachean
+
+abbrev Kripke.FrameClass.trans_mckinsey : FrameClass := { F | IsTrans _ F ∧ SatisfiesMcKinseyCondition _ F }
+
+namespace Hilbert.K4Point1
+
+instance Kripke.sound : Sound (Hilbert.K4Point1) (Kripke.FrameClass.trans_mckinsey) := instSound_of_validates_axioms $ by
+  apply FrameClass.Validates.withAxiomK;
+  rintro F ⟨_, _⟩ _ (rfl | rfl);
+  . exact validate_AxiomFour_of_transitive;
+  . exact validate_axiomM_of_satisfiesMcKinseyCondition;
+
+instance Kripke.consistent : Entailment.Consistent (Hilbert.K4Point1) := consistent_of_sound_frameclass Kripke.FrameClass.trans_mckinsey $ by
+  use whitepoint;
+  apply Set.mem_setOf_eq.mpr;
+  constructor <;> infer_instance;
+
+instance Kripke.canonical : Canonical (Hilbert.K4Point1) Kripke.FrameClass.trans_mckinsey := ⟨by
+  apply Set.mem_setOf_eq.mpr;
+  constructor;
+  . infer_instance;
+  . apply Canonical.satisfiesMcKinseyCondition;
+⟩
+
+instance Kripke.complete : Complete (Hilbert.K4Point1) Kripke.FrameClass.trans_mckinsey := inferInstance
+
+end Hilbert.K4Point1
+
+namespace Logic
+
+open Formula
+open Entailment
+open Kripke
+
+lemma K4Point1.Kripke.trans_mckinsey : Logic.K4Point1 = FrameClass.trans_mckinsey.logic := eq_hilbert_logic_frameClass_logic
+
+instance : ProperSublogic Logic.K4 Logic.K4Point1 := ⟨by
+  constructor;
+  . exact Hilbert.weakerThan_of_dominate_axioms (by simp) |>.subset;
+  . suffices ∃ φ, Hilbert.K4Point1 ⊢! φ ∧ ¬Kripke.FrameClass.trans ⊧ φ by
+      rw [K4.Kripke.trans];
+      tauto;
+    use (Axioms.M (.atom 0));
+    constructor;
+    . exact axiomM!;
+    . apply Kripke.not_validOnFrameClass_of_exists_model_world;
+      use ⟨⟨Fin 1, λ x y => False⟩, λ w _ => False⟩, 0;
+      constructor;
+      . refine ⟨by tauto⟩;
+      . simp [Semantics.Realize, Satisfies];
+⟩
+
+end Logic
+
+
+end LO.Modal
