Foundation/Modal/Kripke/Logic/K4Point3.lean
@@ -1,0 +1,80 @@
+import Foundation.Modal.Kripke.AxiomWeakPoint3
+import Foundation.Modal.Kripke.AxiomGeach
+import Foundation.Modal.Kripke.Hilbert
+import Foundation.Modal.Hilbert.WellKnown
+import Foundation.Modal.Kripke.Logic.K4
+
+namespace LO.Modal
+
+open Kripke
+open Hilbert.Kripke
+open Geachean
+
+abbrev Kripke.FrameClass.trans_weakConnected : FrameClass := { F | IsTrans _ F ∧ IsWeakConnected _ F }
+
+namespace Hilbert.K4Point3.Kripke
+
+instance sound : Sound (Hilbert.K4Point3) Kripke.FrameClass.trans_weakConnected := instSound_of_validates_axioms $ by
+  apply FrameClass.Validates.withAxiomK;
+  rintro F ⟨_, _⟩ _ (rfl | rfl);
+  . exact validate_AxiomFour_of_transitive;
+  . exact validate_WeakPoint3_of_weakConnected;
+
+instance consistent : Entailment.Consistent (Hilbert.K4Point3) :=
+  consistent_of_sound_frameclass FrameClass.trans_weakConnected $ by
+    use whitepoint;
+    apply Set.mem_setOf_eq.mpr;
+    constructor;
+    . infer_instance;
+    . infer_instance;
+
+instance canonical : Canonical (Hilbert.K4Point3) Kripke.FrameClass.trans_weakConnected :=  ⟨by
+  apply Set.mem_setOf_eq.mpr;
+  constructor <;> infer_instance;
+⟩
+
+instance complete : Complete (Hilbert.K4Point3) Kripke.FrameClass.trans_weakConnected := inferInstance
+
+end Hilbert.K4Point3.Kripke
+
+namespace Logic
+
+open Formula
+open Entailment
+open Kripke
+
+lemma K4Point3.Kripke.trans_weakConnected : Logic.K4Point3 = FrameClass.trans_weakConnected.logic := eq_hilbert_logic_frameClass_logic
+
+instance : ProperSublogic Logic.K4 Logic.K4Point3 := ⟨by
+  constructor;
+  . exact Hilbert.weakerThan_of_dominate_axioms (by simp) |>.subset;
+  . suffices ∃ φ, Hilbert.K4Point3 ⊢! φ ∧ ¬Kripke.FrameClass.trans ⊧ φ by
+      rw [K4.Kripke.trans];
+      tauto;
+    use (Axioms.WeakPoint3 (.atom 0) (.atom 1));
+    constructor;
+    . exact axiomWeakPoint3!;
+    . apply Kripke.not_validOnFrameClass_of_exists_model_world;
+      let M : Model := ⟨
+        ⟨Fin 3, λ x y => x = 0 ∧ y ≠ 0⟩,
+        λ w a => if a = 0 then w = 1 else w = 2
+      ⟩;
+      use M, 0;
+      constructor;
+      . refine ⟨by omega⟩
+      . suffices
+          ∃ x : M.World, (0 : M.World) ≺ x ∧ x = 1 ∧ (∀ y, x ≺ y → y = 1) ∧ ¬x = 2 ∧
+          ∃ x : M.World, (0 : M.World) ≺ x ∧ x = 2 ∧ (∀ z : M.World, x ≺ z → z = 2) ∧ x ≠ 1
+          by simpa [M, Semantics.Realize, Satisfies];
+        refine ⟨1, ?_, rfl, ?_, ?_, 2, ?_, rfl, ?_, ?_⟩;
+        . trivial;
+        . omega;
+        . trivial;
+        . omega;
+        . trivial;
+        . trivial;
+⟩
+
+end Logic
+
+end LO.Modal
