Foundation/Modal/Kripke/Logic/KB.lean
@@ -1,0 +1,65 @@
+import Foundation.Modal.Kripke.AxiomGeach
+import Foundation.Modal.Kripke.Hilbert
+import Foundation.Modal.Hilbert.WellKnown
+import Foundation.Modal.Kripke.Logic.K
+
+namespace LO.Modal
+
+open Kripke
+open Hilbert.Kripke
+open Geachean
+
+
+protected abbrev Kripke.FrameClass.symm : FrameClass := { F | IsSymm _ F }
+
+namespace Hilbert.KB.Kripke
+
+instance sound : Sound (Hilbert.KB) Kripke.FrameClass.symm := instSound_of_validates_axioms $ by
+  apply FrameClass.Validates.withAxiomK;
+  rintro F F_symm _ rfl;
+  exact validate_AxiomB_of_symmetric (sym := F_symm);
+
+instance consistent : Entailment.Consistent (Hilbert.KB) := consistent_of_sound_frameclass FrameClass.symm $ by
+  use whitepoint;
+  apply Set.mem_setOf_eq.mpr;
+  infer_instance;
+
+instance canonical : Canonical (Hilbert.KB) Kripke.FrameClass.symm := ⟨by
+  apply Set.mem_setOf_eq.mpr;
+  infer_instance;
+⟩
+
+instance complete : Complete (Hilbert.KB) Kripke.FrameClass.symm := inferInstance
+
+end Hilbert.KB.Kripke
+
+namespace Logic
+
+open Formula
+open Entailment
+open Kripke
+
+lemma KB.Kripke.symm : Logic.KB = FrameClass.symm.logic := eq_hilbert_logic_frameClass_logic
+
+instance : ProperSublogic Logic.K Logic.KB := ⟨by
+  constructor;
+  . exact Hilbert.weakerThan_of_dominate_axioms (by simp) |>.subset;
+  . suffices ∃ φ, Hilbert.KB ⊢! φ ∧ ¬FrameClass.all ⊧ φ by
+      rw [K.Kripke.all];
+      tauto;
+    use (Axioms.B (.atom 0));
+    constructor;
+    . exact axiomB!;
+    . apply Kripke.not_validOnFrameClass_of_exists_model_world;
+      let M : Model := ⟨⟨Fin 2, λ x y => x = 0 ∧ y = 1⟩, λ w _ => w = 0⟩;
+      use M, 0;
+      constructor;
+      . trivial;
+      . suffices ∃ (x : M.World), (0 : M.World) ≺ x ∧ ¬x ≺ 0 by simpa [Semantics.Realize, Satisfies, M];
+        use 1;
+        trivial;
+⟩
+
+end Logic
+
+end LO.Modal
