Foundation/Modal/Kripke/Logic/KB4.lean
@@ -1,0 +1,82 @@
+import Foundation.Modal.Kripke.AxiomGeach
+import Foundation.Modal.Kripke.Hilbert
+import Foundation.Modal.Hilbert.WellKnown
+import Foundation.Modal.Kripke.Logic.K45
+import Foundation.Modal.Kripke.Logic.KB
+
+namespace LO.Modal
+
+open Kripke
+open Hilbert.Kripke
+open Geachean
+
+abbrev Kripke.FrameClass.symm_trans : FrameClass := { F | IsSymm _ F ∧ IsTrans _ F }
+
+namespace Hilbert.KB4.Kripke
+
+instance sound : Sound (Hilbert.KB4) Kripke.FrameClass.symm_trans := instSound_of_validates_axioms $ by
+  apply FrameClass.Validates.withAxiomK;
+  rintro F ⟨_, _⟩ _ (rfl | rfl);
+  . exact validate_AxiomB_of_symmetric;
+  . exact validate_AxiomFour_of_transitive;
+
+instance consistent : Entailment.Consistent (Hilbert.KB4) := consistent_of_sound_frameclass Kripke.FrameClass.symm_trans $ by
+  use whitepoint;
+  constructor <;> infer_instance;
+
+instance canonical : Canonical (Hilbert.KB4) Kripke.FrameClass.symm_trans := ⟨by
+  apply Set.mem_setOf_eq.mpr;
+  constructor <;> infer_instance;
+⟩
+
+instance complete : Complete (Hilbert.KB4) Kripke.FrameClass.symm_trans := inferInstance
+
+end Hilbert.KB4.Kripke
+
+namespace Logic
+
+open Formula
+open Entailment
+open Kripke
+
+lemma KB4.Kripke.refl_trans : Logic.KB4 = FrameClass.symm_trans.logic := eq_hilbert_logic_frameClass_logic
+
+instance : ProperSublogic Logic.K45 Logic.KB4 := ⟨by
+  constructor;
+  . rw [K45.Kripke.trans_eucl, KB4.Kripke.refl_trans];
+    rintro φ hφ F ⟨_, _⟩;
+    apply hφ;
+    refine ⟨inferInstance, inferInstance⟩;
+  . suffices ∃ φ, Hilbert.KB4 ⊢! φ ∧ ¬FrameClass.trans_eucl ⊧ φ by
+      rw [K45.Kripke.trans_eucl];
+      tauto;
+    use Axioms.B (.atom 0);
+    constructor;
+    . exact axiomB!;
+    . apply Kripke.not_validOnFrameClass_of_exists_model_world;
+      use ⟨⟨Fin 2, λ x y => y = 1⟩, λ w _ => w = 0⟩, 0;
+      constructor;
+      . refine ⟨⟨by tauto⟩, ⟨by tauto⟩⟩;
+      . simp [Semantics.Realize, Satisfies];
+⟩
+
+instance : ProperSublogic Logic.KB Logic.KB4 := ⟨by
+  constructor;
+  . exact Hilbert.weakerThan_of_dominate_axioms (by simp) |>.subset;
+  . suffices ∃ φ, Hilbert.KB4 ⊢! φ ∧ ¬FrameClass.symm ⊧ φ by
+      rw [KB.Kripke.symm];
+      tauto;
+    use Axioms.Four (.atom 0);
+    constructor;
+    . exact axiomFour!;
+    . apply Kripke.not_validOnFrameClass_of_exists_model_world;
+      use ⟨⟨Bool, λ x y => x != y⟩, λ w _ => w = true⟩, false;
+      constructor;
+      . refine ⟨by simp⟩;
+      . simp [Semantics.Realize, Satisfies];
+        tauto;
+⟩
+
+end Logic
+
+end LO.Modal
