Foundation/Modal/Kripke/Logic/KD45.lean
@@ -1,0 +1,126 @@
+import Foundation.Modal.Kripke.AxiomGeach
+import Foundation.Modal.Kripke.Hilbert
+import Foundation.Modal.Hilbert.WellKnown
+import Foundation.Modal.Kripke.Logic.KD4
+import Foundation.Modal.Kripke.Logic.KD5
+import Foundation.Modal.Kripke.Logic.K45
+
+namespace LO.Modal
+
+open Kripke
+open Hilbert.Kripke
+open Geachean
+
+abbrev Kripke.FrameClass.serial_trans_eucl : FrameClass := { F | IsSerial _ F ∧ IsTrans _ F ∧ IsEuclidean _ F }
+
+namespace Hilbert.KD45.Kripke
+
+instance sound : Sound (Hilbert.KD45) Kripke.FrameClass.serial_trans_eucl := instSound_of_validates_axioms $ by
+  apply FrameClass.Validates.withAxiomK;
+  rintro F ⟨_, _, _⟩ _ (rfl | rfl | rfl);
+  . exact validate_AxiomD_of_serial;
+  . exact validate_AxiomFour_of_transitive;
+  . exact validate_AxiomFive_of_euclidean;
+
+instance consistent : Entailment.Consistent (Hilbert.KD45) := consistent_of_sound_frameclass Kripke.FrameClass.serial_trans_eucl $ by
+  use whitepoint;
+  refine ⟨inferInstance, inferInstance, inferInstance⟩;
+
+instance canonical : Canonical (Hilbert.KD45) Kripke.FrameClass.serial_trans_eucl := ⟨by
+  apply Set.mem_setOf_eq.mpr;
+  refine ⟨inferInstance, inferInstance, inferInstance⟩;
+⟩
+
+instance complete : Complete (Hilbert.KD45) Kripke.FrameClass.serial_trans_eucl := inferInstance
+
+end Hilbert.KD45.Kripke
+
+namespace Logic
+
+open Formula
+open Entailment
+open Kripke
+
+lemma KD45.Kripke.serial_trans_eucl : Logic.KD45 = FrameClass.serial_trans_eucl.logic := eq_hilbert_logic_frameClass_logic
+
+instance : ProperSublogic Logic.KD4 Logic.KD45 := ⟨by
+  constructor;
+  . exact Hilbert.weakerThan_of_dominate_axioms (by simp) |>.subset;
+  . suffices ∃ φ, Hilbert.KD45 ⊢! φ ∧ ¬FrameClass.serial_trans ⊧ φ by
+      rw [KD4.Kripke.serial_trans];
+      tauto;
+    use Axioms.Five (.atom 0);
+    constructor;
+    . exact axiomFive!;
+    . apply Kripke.not_validOnFrameClass_of_exists_model_world;
+      let M : Model := ⟨
+          ⟨Fin 3, λ x y => x = y ∨ x < y⟩,
+          λ w _ => w = 0
+        ⟩;
+      use M, 0;
+      constructor;
+      . refine ⟨⟨by tauto⟩, ⟨by omega⟩⟩;
+      . suffices (0 : M.World) ≺ 0 ∧ ∃ x : M.World, (0 : M.World) ≺ x ∧ ¬x ≺ 0 by
+          simpa [M, Semantics.Realize, Satisfies];
+        constructor;
+        . tauto;
+        . use 1;
+          constructor <;> omega;
+⟩
+
+instance : ProperSublogic Logic.KD5 Logic.KD45 := ⟨by
+  constructor;
+  . exact Hilbert.weakerThan_of_dominate_axioms (by simp) |>.subset;
+  . suffices ∃ φ, Hilbert.KD45 ⊢! φ ∧ ¬FrameClass.serial_eucl ⊧ φ by
+      rw [KD5.Kripke.serial_eucl];
+      tauto;
+    use (Axioms.Four (.atom 0));
+    constructor;
+    . exact axiomFour!;
+    . apply Kripke.not_validOnFrameClass_of_exists_model_world;
+      let M : Model := ⟨⟨Fin 3, λ x y => (x = 0 ∧ y = 1) ∨ (x ≠ 0 ∧ y ≠ 0)⟩, λ w _ => w = 1⟩;
+      use M, 0;
+      constructor;
+      . refine ⟨⟨?_⟩, ⟨by unfold Euclidean; omega⟩⟩;
+        . intro x;
+          match x with
+          | 0 => use 1; tauto;
+          | 1 => use 1; omega;
+          | 2 => use 2; omega;
+      . suffices (∀ (y : M.World), (0 : M.World) ≺ y → y = 1) ∧ ∃ x, (0 : M.World) ≺ x ∧ ∃ y, x ≺ y ∧ y ≠ 1 by
+          simpa [M, Semantics.Realize, Satisfies];
+        constructor;
+        . intro y;
+          match y with
+          | 0 => tauto;
+          | 1 => tauto;
+          | 2 => tauto;
+        . use 1;
+          constructor;
+          . tauto;
+          . use 2;
+            constructor;
+            . omega;
+            . trivial;
+⟩
+
+instance : ProperSublogic Logic.K45 Logic.KD45 := ⟨by
+  constructor;
+  . exact Hilbert.weakerThan_of_dominate_axioms (by simp) |>.subset;
+  . suffices ∃ φ, Hilbert.KD45 ⊢! φ ∧ ¬FrameClass.trans_eucl ⊧ φ by
+      rw [K45.Kripke.trans_eucl];
+      tauto;
+    use Axioms.D (.atom 0);
+    constructor;
+    . exact axiomD!;
+    . apply Kripke.not_validOnFrameClass_of_exists_model_world;
+      use ⟨⟨Fin 1, λ x y => False⟩, λ w _ => True⟩, 0;
+      constructor;
+      . refine ⟨⟨by tauto⟩, ⟨by tauto⟩⟩;
+      . simp [Semantics.Realize, Satisfies];
+⟩
+
+end Logic
+
+
+end LO.Modal
