Foundation/Modal/Kripke/Logic/KDB.lean
@@ -1,0 +1,85 @@
+import Foundation.Modal.Kripke.AxiomGeach
+import Foundation.Modal.Kripke.Hilbert
+import Foundation.Modal.Hilbert.WellKnown
+import Foundation.Modal.Kripke.Logic.KB
+import Foundation.Modal.Kripke.Logic.KD
+
+namespace LO.Modal
+
+open Kripke
+open Hilbert.Kripke
+open Geachean
+
+abbrev Kripke.FrameClass.serial_symm : FrameClass := { F | IsSerial _ F ∧ IsSymm _ F }
+
+namespace Hilbert.KDB.Kripke
+
+instance sound : Sound (Hilbert.KDB) Kripke.FrameClass.serial_symm := instSound_of_validates_axioms $ by
+  apply FrameClass.Validates.withAxiomK;
+  rintro F ⟨_, _⟩ _ (rfl | rfl);
+  . exact validate_AxiomD_of_serial;
+  . exact validate_AxiomB_of_symmetric;
+
+instance consistent : Entailment.Consistent (Hilbert.KDB) := consistent_of_sound_frameclass Kripke.FrameClass.serial_symm $ by
+  use whitepoint;
+  constructor <;> infer_instance;
+
+instance canonical : Canonical (Hilbert.KDB) Kripke.FrameClass.serial_symm := ⟨by
+  apply Set.mem_setOf_eq.mpr;
+  constructor <;> infer_instance;
+⟩
+
+instance complete : Complete (Hilbert.KDB) Kripke.FrameClass.serial_symm := inferInstance
+
+end Hilbert.KDB.Kripke
+
+namespace Logic
+
+open Formula
+open Entailment
+open Kripke
+
+lemma KDB.Kripke.serial_symm : Logic.KDB = FrameClass.serial_symm.logic := eq_hilbert_logic_frameClass_logic
+
+instance : ProperSublogic Logic.KD Logic.KDB := ⟨by
+  constructor;
+  . exact Hilbert.weakerThan_of_dominate_axioms (by simp) |>.subset;
+  . suffices ∃ φ, Hilbert.KDB ⊢! φ ∧ ¬FrameClass.serial ⊧ φ by
+      rw [KD.Kripke.serial];
+      tauto;
+    use Axioms.B (.atom 0);
+    constructor;
+    . exact axiomB!;
+    . apply Kripke.not_validOnFrameClass_of_exists_model_world;
+      let M : Model := ⟨⟨Fin 2, λ x y => x ≤ y⟩, λ w _ => w = 0⟩;
+      use M, 0;
+      constructor;
+      . refine ⟨?_⟩;
+        intro x;
+        match x with
+        | 0 => use 1; tauto;
+        | 1 => use 1;
+      . suffices ∃ x, (0 : M.World) ≺ x ∧ ¬x ≺ 0 by simpa [M, Semantics.Realize, Satisfies];
+        use 1;
+        constructor <;> omega;
+⟩
+
+instance : ProperSublogic Logic.KB Logic.KDB := ⟨by
+  constructor;
+  . exact Hilbert.weakerThan_of_dominate_axioms (by simp) |>.subset;
+  . suffices ∃ φ, Hilbert.KDB ⊢! φ ∧ ¬FrameClass.symm ⊧ φ by
+      rw [KB.Kripke.symm];
+      tauto;
+    use Axioms.D (.atom 0);
+    constructor;
+    . exact axiomD!;
+    . apply Kripke.not_validOnFrameClass_of_exists_model_world;
+      use ⟨⟨Fin 1, λ x y => False⟩, λ w _ => w = 0⟩, 0;
+      constructor;
+      . refine ⟨by tauto⟩;
+      . simp [Semantics.Realize, Satisfies];
+⟩
+
+end Logic
+
+end LO.Modal
