Foundation/Modal/Kripke/Logic/KTc.lean
@@ -1,0 +1,69 @@
+import Foundation.Modal.Kripke.AxiomGeach
+import Foundation.Modal.Kripke.Hilbert
+import Foundation.Modal.Hilbert.WellKnown
+import Foundation.Modal.Kripke.Logic.KB4
+
+namespace LO.Modal
+
+open Kripke
+open Hilbert.Kripke
+open Geachean
+
+protected abbrev Kripke.FrameClass.corefl : FrameClass := { F | IsCoreflexive _ F.Rel }
+
+namespace Hilbert.KTc.Kripke
+
+instance sound : Sound (Hilbert.KTc) Kripke.FrameClass.corefl := instSound_of_validates_axioms $ by
+  apply FrameClass.Validates.withAxiomK;
+  rintro F F_corefl _ rfl;
+  exact Kripke.validate_AxiomTc_of_coreflexive (corefl := F_corefl);
+
+instance consistent : Entailment.Consistent (Hilbert.KTc) := consistent_of_sound_frameclass Kripke.FrameClass.corefl $ by
+  use whitepoint;
+  apply Set.mem_setOf_eq.mpr;
+  infer_instance;
+
+instance canonical : Canonical (Hilbert.KTc) FrameClass.corefl := ⟨by
+  apply Set.mem_setOf_eq.mpr;
+  infer_instance;
+⟩
+
+instance complete : Complete (Hilbert.KTc) FrameClass.corefl := inferInstance
+
+end Hilbert.KTc.Kripke
+
+namespace Logic
+
+open Formula
+open Entailment
+open Kripke
+
+lemma KTc.Kripke.corefl : Logic.KTc = FrameClass.corefl.logic := eq_hilbert_logic_frameClass_logic
+
+instance : ProperSublogic Logic.KB4 Logic.KTc := ⟨by
+  constructor;
+  . rw [KB4.Kripke.refl_trans, KTc.Kripke.corefl];
+    rintro φ hφ F F_corefl;
+    replace hF := Set.mem_setOf_eq.mp F_corefl;
+    apply hφ;
+    refine ⟨inferInstance, inferInstance⟩;
+  . suffices ∃ φ, Hilbert.KTc ⊢! φ ∧ ¬Kripke.FrameClass.symm_trans ⊧ φ by
+      rw [KB4.Kripke.refl_trans];
+      tauto;
+    use (Axioms.Tc (.atom 0));
+    constructor;
+    . exact axiomTc!;
+    . apply Kripke.not_validOnFrameClass_of_exists_model_world;
+      let M : Model := ⟨⟨Fin 2, λ x y => True⟩, λ w _ => w = 0⟩;
+      use M, 0;
+      constructor;
+      . refine ⟨⟨by simp [M]⟩, ⟨by simp [M]⟩⟩
+      . suffices ∃ x, (x : M.World) ≠ 0 by
+          simp [M, Semantics.Realize, Satisfies];
+          tauto;
+        use 1;
+        aesop;
+⟩
+end Logic
+
+end LO.Modal
