Foundation/Modal/Kripke/Logic/S4.lean
@@ -1,0 +1,119 @@
+import Foundation.Modal.Entailment.KT
+import Foundation.Modal.Kripke.Filtration
+import Foundation.Modal.Kripke.Logic.KD4
+import Foundation.Modal.Kripke.Logic.KT
+
+namespace LO.Modal
+
+open Kripke
+open Hilbert.Kripke
+open Geachean
+
+
+namespace Kripke
+
+protected abbrev FrameClass.preorder : FrameClass := { F | IsPreorder _ F }
+
+protected abbrev FrameClass.finite_preorder: FrameClass := { F | Finite F.World ∧ IsPreorder _ F.Rel }
+
+end Kripke
+
+
+namespace Hilbert.S4.Kripke
+
+instance sound : Sound (Hilbert.S4) Kripke.FrameClass.preorder := instSound_of_validates_axioms $ by
+  apply FrameClass.Validates.withAxiomK;
+  rintro F ⟨_, _⟩ _ (rfl | rfl);
+  . exact validate_AxiomT_of_reflexive;
+  . exact validate_AxiomFour_of_transitive;
+
+instance consistent : Entailment.Consistent (Hilbert.S4) := consistent_of_sound_frameclass Kripke.FrameClass.preorder $ by
+  use whitepoint;
+  constructor;
+
+instance canonical : Canonical (Hilbert.S4) Kripke.FrameClass.preorder := ⟨by
+  apply Set.mem_setOf_eq.mpr;
+  constructor;
+⟩
+
+instance complete : Complete (Hilbert.S4) Kripke.FrameClass.preorder := inferInstance
+
+open finestFiltrationTransitiveClosureModel in
+instance finiteComplete : Complete (Hilbert.S4) Kripke.FrameClass.finite_preorder := ⟨by
+  intro φ hp;
+  apply Kripke.complete.complete;
+  rintro F F_preorder V x;
+  replace F_preorder := Set.mem_setOf_eq.mp F_preorder;
+  let M : Kripke.Model := ⟨F, V⟩;
+  let FM := finestFiltrationTransitiveClosureModel M φ.subformulas;
+  apply filtration FM (finestFiltrationTransitiveClosureModel.filterOf) (by subformula) |>.mpr;
+  apply hp;
+  refine ⟨?_, ?_⟩;
+  . apply FilterEqvQuotient.finite;
+    simp;
+  . exact finestFiltrationTransitiveClosureModel.isPreorder;
+⟩
+
+end Hilbert.S4.Kripke
+
+namespace Logic
+
+open Formula
+open Entailment
+open Kripke
+
+lemma S4.Kripke.preorder : Logic.S4 = FrameClass.preorder.logic := eq_hilbert_logic_frameClass_logic
+
+instance : ProperSublogic Logic.KT Logic.S4 := ⟨by
+  constructor;
+  . exact Hilbert.weakerThan_of_dominate_axioms (by simp [axiomK!, axiomT!]) |>.subset;
+  . suffices ∃ φ, Hilbert.S4 ⊢! φ ∧ ¬Kripke.FrameClass.refl ⊧ φ by
+      rw [KT.Kripke.refl];
+      tauto;
+    use Axioms.Four (.atom 0);
+    constructor;
+    . exact axiomFour!;
+    . apply Kripke.not_validOnFrameClass_of_exists_model_world;
+      let M : Model := ⟨
+          ⟨Fin 3, λ x y => (x = 0 ∧ y ≠ 2) ∨ (x = 1 ∧ y ≠ 0) ∨ (x = 2 ∧ y = 2)⟩,
+          λ w _ => w = 0 ∨ w = 1
+        ⟩;
+      use M, 0;
+      constructor;
+      . refine ⟨by omega⟩;
+      . suffices (∀ (y : M.World), (0 : M.World) ≺ y → y = 0 ∨ y = 1) ∧ ∃ x, (0 : M.World) ≺ x ∧ ∃ y, x ≺ y ∧ y ≠ 0 ∧ y ≠ 1 by
+          simpa [M, Semantics.Realize, Satisfies];
+        constructor;
+        . intro y hy;
+          match y with
+          | 0 => tauto;
+          | 1 => tauto;
+          | 2 => omega;
+        . use 1;
+          constructor;
+          . omega;
+          . use 2;
+            refine ⟨by omega;, by trivial, by trivial⟩;
+⟩
+
+instance : ProperSublogic Logic.KD4 Logic.S4 := ⟨by
+  constructor;
+  . exact Hilbert.weakerThan_of_dominate_axioms (by simp) |>.subset;
+  . suffices ∃ φ, Hilbert.S4 ⊢! φ ∧ ¬FrameClass.serial_trans ⊧ φ by
+      rw [KD4.Kripke.serial_trans];
+      tauto;
+    use Axioms.T (.atom 0);
+    constructor;
+    . exact axiomT!;
+    . apply Kripke.not_validOnFrameClass_of_exists_model_world;
+      use ⟨⟨Fin 3, λ _ y => y = 1⟩, (λ w _ => w = 1)⟩, 0;
+      constructor;
+      . refine ⟨⟨by tauto⟩, ⟨by omega⟩⟩;
+      . simp [Semantics.Realize, Satisfies];
+⟩
+
+instance : ProperSublogic Logic.KD Logic.S4 := ProperSublogic.trans Logic.KD Logic.KT Logic.S4
+
+end Logic
+
+end LO.Modal
