Foundation/Modal/Kripke/Logic/S4Point3.lean
@@ -1,0 +1,198 @@
+import Foundation.Modal.Kripke.Logic.S4
+import Foundation.Modal.Kripke.AxiomPoint3
+import Foundation.Modal.Kripke.Filtration
+import Foundation.Modal.Kripke.Rooted
+import Foundation.Modal.Kripke.Logic.S4Point2
+import Foundation.Modal.Kripke.Logic.K4Point3
+
+namespace LO.Modal
+
+open Kripke
+open Hilbert.Kripke
+open Geachean
+
+abbrev Kripke.FrameClass.connected_preorder : FrameClass := { F | IsPreorder _ F ∧ IsConnected _ F }
+abbrev Kripke.FrameClass.finite_connected_preorder : FrameClass := { F | F.IsFinite ∧ IsPreorder _ F ∧ IsConnected _ F }
+
+/-
+namespace Kripke.FrameClass.connected_preorder
+
+@[simp]
+protected lemma nonempty : Kripke.FrameClass.connected_preorder.Nonempty := by
+  use whitepoint;
+  simp [Reflexive, Transitive, Connected];
+
+lemma validates_HilbertS4Point3 : Kripke.FrameClass.connected_preorder.Validates Hilbert.S4Point3.axioms := by
+  apply FrameClass.Validates.withAxiomK;
+  rintro F ⟨_, _, _⟩ _ (rfl | rfl | rfl);
+  . exact validate_AxiomT_of_reflexive $ by assumption
+  . exact validate_AxiomFour_of_transitive $ by assumption;
+  . exact validate_AxiomPoint3_of_connected $ by assumption;
+
+end Kripke.FrameClass.connected_preorder
+-/
+
+namespace Hilbert.S4Point3.Kripke
+
+instance sound : Sound (Hilbert.S4Point3) Kripke.FrameClass.connected_preorder := instSound_of_validates_axioms $ by
+  apply FrameClass.Validates.withAxiomK;
+  rintro F ⟨_, _⟩ _ (rfl | rfl | rfl);
+  . exact validate_AxiomT_of_reflexive;
+  . exact validate_AxiomFour_of_transitive;
+  . exact validate_AxiomPoint3_of_connected;
+
+instance consistent : Entailment.Consistent (Hilbert.S4Point3) :=
+  consistent_of_sound_frameclass FrameClass.connected_preorder $ by
+    use whitepoint;
+    refine ⟨inferInstance, inferInstance⟩;
+
+instance canonical : Canonical (Hilbert.S4Point3) Kripke.FrameClass.connected_preorder := ⟨by
+  apply Set.mem_setOf_eq.mpr;
+  constructor <;> infer_instance;
+⟩
+
+instance complete : Complete (Hilbert.S4Point3) Kripke.FrameClass.connected_preorder := inferInstance
+
+
+section FFP
+
+open
+  finestFiltrationTransitiveClosureModel
+  Relation
+
+instance finite_sound : Sound (Hilbert.S4Point3) Kripke.FrameClass.finite_connected_preorder := instSound_of_validates_axioms $ by
+  apply FrameClass.Validates.withAxiomK;
+  rintro F ⟨_, _, _⟩ _ (rfl | rfl | rfl);
+  . exact validate_AxiomT_of_reflexive;
+  . exact validate_AxiomFour_of_transitive;
+  . exact validate_AxiomPoint3_of_connected;
+
+instance finite_complete : Complete (Hilbert.S4Point3) Kripke.FrameClass.finite_connected_preorder := ⟨by
+  intro φ hφ;
+  apply Kripke.complete.complete;
+  rintro F ⟨_, _⟩ V r;
+  let M : Kripke.Model := ⟨F, V⟩;
+  let RM := M↾r;
+  apply Model.pointGenerate.modal_equivalent_at_root (M := M) (r := r) |>.mp;
+
+  let FRM := finestFiltrationTransitiveClosureModel RM (φ.subformulas);
+  apply filtration FRM (finestFiltrationTransitiveClosureModel.filterOf (trans := Frame.pointGenerate.isTrans)) (by subformula) |>.mpr;
+  apply hφ;
+
+  refine ⟨?_, ?_, ?_⟩;
+  . apply Frame.isFinite_iff _ |>.mpr
+    apply FilterEqvQuotient.finite;
+    simp;
+  . exact finestFiltrationTransitiveClosureModel.isPreorder (preorder := Frame.pointGenerate.isPreorder);
+  . apply isConnected_iff _ _ |>.mpr;
+    rintro X ⟨y, (rfl | Rry)⟩ ⟨z, (rfl | Rrz)⟩ ⟨RXY, RXZ⟩;
+    . simp only [or_self];
+      apply Relation.TransGen.single;
+      suffices z ≺ z by tauto;
+      apply IsRefl.refl;
+    . left;
+      apply Relation.TransGen.single;
+      suffices y ≺ z by tauto;
+      exact Rrz.unwrap;
+    . right;
+      apply Relation.TransGen.single;
+      suffices z ≺ y by tauto;
+      exact Rry.unwrap;
+    . replace Rry := Rry.unwrap;
+      replace Rrz := Rrz.unwrap;
+      rcases IsConnected.connected ⟨Rry, Rrz⟩ with (Ryz | Rrw);
+      . left;
+        apply Relation.TransGen.single;
+        tauto;
+      . right;
+        apply Relation.TransGen.single;
+        tauto;
+⟩
+
+end FFP
+
+end Hilbert.S4Point3.Kripke
+
+namespace Logic
+
+open Formula
+open Entailment
+open Kripke
+
+lemma S4Point3.Kripke.connected_preorder : Logic.S4Point3 = FrameClass.connected_preorder.logic := eq_hilbert_logic_frameClass_logic
+lemma S4Point3.Kripke.finite_connected_preorder : Logic.S4Point3 = FrameClass.finite_connected_preorder.logic := eq_hilbert_logic_frameClass_logic
+
+instance : ProperSublogic Logic.S4Point2 Logic.S4Point3 := ⟨
+  by
+  constructor;
+  . rw [S4Point2.Kripke.confluent_preorder, S4Point3.Kripke.connected_preorder];
+    rintro φ hφ F ⟨_, _⟩;
+    apply hφ;
+    refine ⟨inferInstance, inferInstance⟩;
+  . suffices ∃ φ, Hilbert.S4Point3 ⊢! φ ∧ ¬FrameClass.confluent_preorder ⊧ φ by
+      rw [S4Point2.Kripke.confluent_preorder];
+      tauto;
+    use Axioms.Point3 (.atom 0) (.atom 1);
+    constructor;
+    . exact axiomPoint3!;
+    . apply Kripke.not_validOnFrameClass_of_exists_model_world;
+      let M : Model := ⟨
+        ⟨Fin 4, λ x y => ¬(x = 1 ∧ y = 2) ∧ ¬(x = 2 ∧ y = 1) ∧ (x ≤ y)⟩,
+        λ w a => (a = 0 ∧ (w = 1 ∨ w = 3)) ∨ (a = 1 ∧ (w = 2 ∨ w = 3))
+      ⟩;
+      use M, 0;
+      constructor;
+      . apply Set.mem_setOf_eq.mpr
+        refine ⟨?_, ⟨?_⟩⟩;
+        . apply isPreorder_iff _ _ |>.mpr;
+          refine ⟨⟨by omega⟩, ⟨by omega⟩⟩;
+        . rintro x y z ⟨Rxy, Ryz⟩;
+          use 3;
+          constructor <;> omega;
+      . apply Kripke.Satisfies.or_def.not.mpr;
+        push_neg;
+        constructor;
+        . apply Kripke.Satisfies.box_def.not.mpr;
+          push_neg;
+          use 1;
+          simp [Satisfies, Semantics.Realize, M];
+          constructor <;> omega;
+        . apply Kripke.Satisfies.box_def.not.mpr;
+          push_neg;
+          use 2;
+          simp [Satisfies, Semantics.Realize, M];
+          constructor <;> omega;
+⟩
+
+instance : ProperSublogic Logic.S4 Logic.S4Point3 := ProperSublogic.trans Logic.S4 Logic.S4Point2 Logic.S4Point3
+
+instance : ProperSublogic Logic.K4Point3 Logic.S4Point3 := ⟨by
+  constructor;
+  . rw [K4Point3.Kripke.trans_weakConnected, S4Point3.Kripke.connected_preorder];
+    rintro φ hφ F ⟨_, _⟩;
+    apply hφ;
+    refine ⟨inferInstance, inferInstance⟩;
+  . suffices ∃ φ, Hilbert.S4Point3 ⊢! φ ∧ ¬Kripke.FrameClass.trans_weakConnected ⊧ φ by
+      rw [K4Point3.Kripke.trans_weakConnected];
+      tauto;
+    use (Axioms.Point3 (.atom 0) (.atom 1));
+    constructor;
+    . exact axiomPoint3!;
+    . apply Kripke.not_validOnFrameClass_of_exists_model_world;
+      let M : Model := ⟨
+        ⟨Fin 2, λ x y => x < y⟩,
+        λ w a => False
+      ⟩;
+      use M, 0;
+      constructor;
+      . refine ⟨⟨by omega⟩, ⟨by simp [M, WeakConnected]⟩⟩
+      . suffices ∃ x, (0 : M.World) ≺ x ∧ (∀ y, ¬x ≺ y) ∧ ∃ x, (0 : M.World) ≺ x ∧ ∀ y, ¬x ≺ y by
+          simpa [M, Semantics.Realize, Satisfies];
+        use 1;
+        refine ⟨?_, ?_, ⟨1, ?_, ?_⟩⟩;
+        repeat omega;
+⟩
+
+end Logic
+
+end LO.Modal
