Foundation/Modal/Kripke/Logic/S5Grz.lean
@@ -1,0 +1,63 @@
+import Foundation.Modal.Hilbert.S5Grz
+import Foundation.Modal.Kripke.Logic.Grz.Completeness
+import Foundation.Modal.Kripke.Logic.Triv
+import Foundation.Modal.Kripke.Logic.S5
+
+namespace LO.Modal.Logic
+
+open Formula
+open Entailment
+open Kripke
+
+lemma S5Grz.Kripke.finite_equality : Logic.S5Grz = Kripke.FrameClass.finite_equality.logic := by
+  rw [eq_S5Grz_Triv, Triv.Kripke.finite_equality]
+
+instance : ProperSublogic Logic.S5 Logic.S5Grz := ⟨by
+  constructor;
+  . exact Hilbert.weakerThan_of_dominate_axioms (by simp) |>.subset;
+  . suffices ∃ φ, Hilbert.S5Grz ⊢! φ ∧ ¬FrameClass.universal ⊧ φ by
+      rw [S5.Kripke.universal];
+      tauto;
+    use Axioms.Grz (.atom 0);
+    constructor;
+    . exact axiomGrz!;
+    . apply Kripke.not_validOnFrameClass_of_exists_model_world;
+      use ⟨⟨Fin 2, λ x y => True⟩, λ w _ => w = 1⟩, 0;
+      constructor;
+      . refine ⟨by simp [Universal]⟩;
+      . simp [Semantics.Realize, Satisfies];
+⟩
+
+instance : ProperSublogic Logic.Grz Logic.S5Grz := ⟨by
+  constructor;
+  . exact Hilbert.weakerThan_of_dominate_axioms (by simp) |>.subset;
+  . suffices ∃ φ, Hilbert.S5Grz ⊢! φ ∧ ¬FrameClass.finite_partial_order ⊧ φ by
+      rw [Grz.Kripke.finite_partial_order];
+      tauto;
+    use Axioms.Five (.atom 0)
+    constructor;
+    . exact axiomFive!;
+    . apply Kripke.not_validOnFrameClass_of_exists_model_world;
+      let M : Model := ⟨⟨Fin 2, λ x y => x ≤ y⟩, (λ w _ => w = 0)⟩;
+      use M, 0;
+      constructor;
+      . refine ⟨by tauto, {
+          refl := by omega,
+          trans := by omega;
+          antisymm := by simp [M]; omega;
+        }⟩;
+      . suffices (0 : M.World) ≺ 0 ∧ ∃ x, (0 : M.World) ≺ x ∧ ¬x ≺ 0 by
+          simpa [Semantics.Realize, Satisfies, ValidOnFrame, M];
+        constructor;
+        . omega;
+        . use 1;
+          constructor <;> omega;
+⟩
+
+instance : ProperSublogic Logic.S5 Logic.Triv := by
+  rw [←eq_S5Grz_Triv];
+  infer_instance;
+
+instance : ProperSublogic Logic.S4 Logic.Triv := ProperSublogic.trans Logic.S4 Logic.S5 Logic.Triv
+
+end LO.Modal.Logic
