Foundation/Modal/Kripke/Logic/Ver.lean
@@ -1,0 +1,129 @@
+import Foundation.Modal.Kripke.AxiomVer
+import Foundation.Modal.Hilbert.WellKnown
+import Foundation.Modal.Kripke.Rooted
+import Foundation.Modal.Kripke.Hilbert
+import Foundation.Modal.Kripke.Logic.KTc
+import Foundation.Modal.Kripke.Logic.GLPoint3
+
+namespace LO.Modal
+
+open Kripke
+open Hilbert.Kripke
+
+protected abbrev Kripke.FrameClass.isolated : FrameClass := { F | IsIsolated _ F }
+protected abbrev Kripke.FrameClass.finite_isolated : FrameClass := { F | Finite F.World ∧ IsIsolated _ F }
+
+namespace Hilbert.Ver.Kripke
+
+instance sound : Sound (Hilbert.Ver) FrameClass.isolated := instSound_of_validates_axioms $ by
+  apply FrameClass.Validates.withAxiomK;
+  rintro F hF _ (rfl | rfl);
+  have := Set.mem_setOf_eq.mp hF;
+  exact Kripke.validate_AxiomVer_of_isolated (F := F);
+
+instance sound_finite_isolated : Sound (Hilbert.Ver) Kripke.FrameClass.finite_isolated :=
+  instSound_of_validates_axioms $ by
+    apply FrameClass.Validates.withAxiomK;
+    rintro F ⟨_, _⟩ _ (rfl | rfl);
+    exact validate_AxiomVer_of_isolated (F := F);
+
+instance consistent : Entailment.Consistent (Hilbert.Ver) := consistent_of_sound_frameclass FrameClass.isolated $ by
+  use blackpoint;
+  apply Set.mem_setOf_eq.mpr;
+  infer_instance;
+
+instance : Kripke.Canonical (Hilbert.Ver) FrameClass.isolated := ⟨by
+  apply Set.mem_setOf_eq.mpr;
+  infer_instance;
+⟩
+
+instance complete : Complete (Hilbert.Ver) FrameClass.isolated := inferInstance
+
+instance complete_finite_isolated : Complete (Hilbert.Ver) Kripke.FrameClass.finite_isolated := ⟨by
+  intro φ hφ;
+  apply Kripke.complete.complete;
+  intro F ⟨F_iso⟩ V r;
+  apply Model.pointGenerate.modal_equivalent_at_root (r := r) |>.mp;
+  apply hφ;
+  refine ⟨?_, ?_⟩;
+  . apply finite_iff_exists_equiv_fin.mpr;
+    use 1;
+    constructor;
+    trans Unit;
+    . refine ⟨λ _ => (), λ _ => ⟨r, by tauto⟩, ?_, ?_⟩
+      . simp [Function.LeftInverse];
+        intro x Rrx;
+        exfalso;
+        induction Rrx with
+        | single h => exact F_iso h;
+        | tail _ h => exact F_iso h;
+      . simp [Function.RightInverse, Function.LeftInverse];
+    . exact finOneEquiv.symm;
+  . apply isIsolated_iff _ _ |>.mpr;
+    rintro ⟨x, (rfl | hx)⟩ ⟨y, (rfl | hy)⟩ <;> apply F_iso;
+⟩
+
+end Hilbert.Ver.Kripke
+
+namespace Logic
+
+open Formula
+open Entailment
+open Kripke
+
+lemma Ver.Kripke.isolated : Logic.Ver = FrameClass.isolated.logic := eq_hilbert_logic_frameClass_logic
+lemma Ver.Kripke.finite_isolated : Logic.Ver = FrameClass.finite_isolated.logic := eq_hilbert_logic_frameClass_logic
+
+instance : ProperSublogic Logic.KTc Logic.Ver := ⟨by
+  constructor;
+  . rw [KTc.Kripke.corefl, Ver.Kripke.isolated];
+    rintro φ hφ F hF;
+    replace hF := Set.mem_setOf_eq.mp hF;
+    apply hφ;
+    apply Set.mem_setOf_eq.mpr;
+    infer_instance;
+  . suffices ∃ φ, Hilbert.Ver ⊢! φ ∧ ¬FrameClass.corefl ⊧ φ by
+      rw [KTc.Kripke.corefl];
+      tauto;
+    use (Axioms.Ver ⊥);
+    constructor;
+    . exact axiomVer!;
+    . apply Kripke.not_validOnFrameClass_of_exists_model_world;
+      let M : Model := ⟨⟨Fin 1, λ x y => True⟩, λ w _ => False⟩;
+      use M, 0;
+      constructor;
+      . refine ⟨by unfold Coreflexive; trivial⟩
+      . suffices ∃ x, (0 : M.World) ≺ x by simpa [Satisfies, Semantics.Realize];
+        use 0;
+⟩
+
+instance : ProperSublogic Logic.GLPoint3 Logic.Ver := ⟨by
+  constructor;
+  . rw [GLPoint3.Kripke.finite_strict_linear_order, Ver.Kripke.finite_isolated];
+    rintro φ hφ F ⟨_, _⟩;
+    apply hφ;
+    refine ⟨by tauto, inferInstance, inferInstance⟩;
+  . suffices ∃ φ, Hilbert.Ver ⊢! φ ∧ ¬FrameClass.finite_strict_linear_order ⊧ φ by
+      rw [GLPoint3.Kripke.finite_strict_linear_order];
+      tauto;
+    use (Axioms.Ver ⊥);
+    constructor;
+    . simp;
+    . apply Kripke.not_validOnFrameClass_of_exists_model_world;
+      use ⟨⟨Fin 2, λ x y => x < y⟩, (λ w a => False)⟩, 0;
+      constructor;
+      . refine ⟨inferInstance, {irrefl := ?_, trans := ?_}, ⟨?_⟩⟩;
+        . omega;
+        . omega;
+        . simp [WeakConnected];
+      . simp only [Semantics.Realize, Satisfies, imp_false, not_forall, not_not];
+        use 1;
+        tauto;
+⟩
+
+instance : ProperSublogic Logic.Ver Logic.Univ := inferInstance
+
+end Logic
+
+
+end LO.Modal
