Foundation/Modal/Logic/GL/Independency.lean
@@ -1,6 +1,6 @@
 import Foundation.Modal.Maximal.Unprovability
-import Foundation.Modal.Kripke.Hilbert.GL.MDP
-import Foundation.Modal.Logic.WellKnown
+import Foundation.Modal.Kripke.Logic.GL.MDP
+
 
 namespace LO.Modal
 
